progress de_bruijn variables

BoogieLang/Semantics.thy
@@ -1,5 +1,5 @@
 theory Semantics
-imports Lang Binders
+imports Lang DeBruijn
 begin
 
 datatype 'a val = LitV lit | AbsV 'a  
@@ -113,7 +113,7 @@ type_synonym 'a ty_absval_rel = "'a \<Rightarrow> tcon_id \<Rightarrow> ty list 
 
 fun ty_val_rel :: "'a ty_absval_rel \<Rightarrow> 'a val \<Rightarrow> ty \<Rightarrow> bool"
   where 
-   "ty_val_rel A (LitV v) typ = (typ = TPrim (type_of_lit v))"
+   "ty_val_rel A (LitV v) (TPrim tp) = (tp = (type_of_lit v))"
  | "ty_val_rel A (AbsV v) (TCon c ty_args) = A v c ty_args"
  | "ty_val_rel A _ _ = False"
 
@@ -140,142 +140,141 @@ inductive red_expr :: "'a ty_absval_rel \<Rightarrow> 'a fun_context \<Rightarro
     "\<lbrakk> A,\<Gamma> \<turnstile> \<langle>e, n_s\<rangle> \<Down> v; A,\<Gamma> \<turnstile> \<langle>es, n_s\<rangle> [\<Down>] vs \<rbrakk> \<Longrightarrow>
       A,\<Gamma> \<turnstile> \<langle>(e # es), n_s\<rangle> [\<Down>] (v # vs)"
   | RedForAllTrue:
-    "\<lbrakk>\<And>v. ty_val_rel A v ty \<Longrightarrow> A,\<Gamma> \<turnstile> \<langle>eopen 0 v e, n_s\<rangle> \<Down> LitV (LBool True) \<rbrakk> \<Longrightarrow> 
-     A,\<Gamma> \<turnstile> \<langle>Forall ty e, n_s\<rangle> \<Down> LitV (LBool True)"
-(*  
-| RedForAllTrue:
-    "\<lbrakk>\<And>v. ty_val_rel A v ty \<Longrightarrow> A,\<Gamma> \<turnstile> \<langle>eopen 0 (Val v) e, n_s\<rangle> \<Down> LitV (LBool True) \<rbrakk> \<Longrightarrow> 
+    "\<lbrakk>\<And>v. ty_val_rel A v ty \<Longrightarrow> A,\<Gamma> \<turnstile> \<langle>e, (shift n_s)(0 \<mapsto> v)\<rangle> \<Down> LitV (LBool True) \<rbrakk> \<Longrightarrow> 
      A,\<Gamma> \<turnstile> \<langle>Forall ty e, n_s\<rangle> \<Down> LitV (LBool True)"
   | RedForAllFalse:
-    "\<lbrakk>ty_val_rel A v ty;  A,\<Gamma> \<turnstile> \<langle>eopen 0 (Val v) e, n_s\<rangle> \<Down> LitV (LBool False) \<rbrakk> \<Longrightarrow> 
+    "\<lbrakk>ty_val_rel A v ty;  A,\<Gamma> \<turnstile> \<langle>e, (shift n_s)(0 \<mapsto> v)\<rangle> \<Down> LitV (LBool False) \<rbrakk> \<Longrightarrow> 
      A,\<Gamma> \<turnstile> \<langle>Forall ty e, n_s\<rangle> \<Down> LitV (LBool False)"
   | RedExistsTrue:
-    "\<lbrakk>ty_val_rel A v ty; A,\<Gamma> \<turnstile> \<langle>eopen 0 (Val v) e, n_s\<rangle> \<Down> LitV (LBool True) \<rbrakk> \<Longrightarrow>
+    "\<lbrakk>ty_val_rel A v ty; A,\<Gamma> \<turnstile> \<langle>e, (shift n_s)(0 \<mapsto> v)\<rangle> \<Down> LitV (LBool True) \<rbrakk> \<Longrightarrow>
      A,\<Gamma> \<turnstile> \<langle>Exists ty e, n_s\<rangle> \<Down> LitV (LBool True)"
   | RedExistsFalse:
-    "\<lbrakk>\<And>v. ty_val_rel A v ty \<Longrightarrow> A,\<Gamma> \<turnstile> \<langle>eopen 0 (Val v) e, n_s\<rangle> \<Down> LitV (LBool False) \<rbrakk> \<Longrightarrow>
+    "\<lbrakk>\<And>v. ty_val_rel A v ty \<Longrightarrow> A,\<Gamma> \<turnstile> \<langle>e, (shift n_s)(0 \<mapsto> v)\<rangle> \<Down> LitV (LBool False) \<rbrakk> \<Longrightarrow>
      A,\<Gamma> \<turnstile> \<langle>Exists ty e, n_s\<rangle> \<Down> LitV (LBool False)"
-*)
 
-inductive_cases RedBinOp_case[elim!]: "\<Gamma> \<turnstile> \<langle>(e1 \<guillemotleft>bop\<guillemotright> e2), n_s\<rangle> \<Down> v"
-inductive_cases RedUnOp_case[elim!]: "\<Gamma> \<turnstile> \<langle>UnOp uop e1, n_s\<rangle> \<Down> v"
-inductive_cases RedFunOp_case[elim!]: "\<Gamma> \<turnstile> \<langle> FunExp f args, n_s \<rangle> \<Down> v"
-inductive_cases RedVal_case[elim]: "\<Gamma> \<turnstile> \<langle>(Val v), n_s\<rangle> \<Down> v"
-inductive_cases RedVar_case[elim!]: "\<Gamma> \<turnstile> \<langle>(Var x), n_s\<rangle> \<Down> v"
-inductive_cases RedForAllTrue_case: "\<Gamma> \<turnstile> \<langle>Forall ty e, n_s\<rangle> \<Down> LBool True"
-inductive_cases RedForAllFalse_case: "\<Gamma> \<turnstile> \<langle>Forall ty e, n_s\<rangle> \<Down> LBool False"
 
-inductive red_cmd :: "var_context \<Rightarrow> fun_context \<Rightarrow> cmd \<Rightarrow> state \<Rightarrow> state \<Rightarrow> bool"
-  ("_,_ \<turnstile> ((\<langle>_,_\<rangle>) \<rightarrow>/ _)" [51,51,0,0,0] 81)
-  for \<Lambda> :: var_context and \<Gamma> :: fun_context
+inductive_cases RedBinOp_case[elim!]: "A,\<Gamma> \<turnstile> \<langle>(e1 \<guillemotleft>bop\<guillemotright> e2), n_s\<rangle> \<Down> v"
+inductive_cases RedUnOp_case[elim!]: "A,\<Gamma> \<turnstile> \<langle>UnOp uop e1, n_s\<rangle> \<Down> v"
+inductive_cases RedFunOp_case[elim!]: "A,\<Gamma> \<turnstile> \<langle> FunExp f args, n_s \<rangle> \<Down> v"
+inductive_cases RedVal_case[elim]: "A,\<Gamma> \<turnstile> \<langle>(Val v), n_s\<rangle> \<Down> v"
+inductive_cases RedVar_case[elim!]: "A,\<Gamma> \<turnstile> \<langle>(Var x), n_s\<rangle> \<Down> v"
+inductive_cases RedForAllTrue_case: "A,\<Gamma> \<turnstile> \<langle>Forall ty e, n_s\<rangle> \<Down> LitV (LBool True)"
+inductive_cases RedForAllFalse_case: "A,\<Gamma> \<turnstile> \<langle>Forall ty e, n_s\<rangle> \<Down> LitV (LBool False)"
+
+inductive red_cmd :: "'a ty_absval_rel \<Rightarrow> var_context \<Rightarrow> 'a fun_context \<Rightarrow> cmd \<Rightarrow> 'a state \<Rightarrow> 'a state \<Rightarrow> bool"
+  ("_,_,_ \<turnstile> ((\<langle>_,_\<rangle>) \<rightarrow>/ _)" [51,51,0,0,0] 81)
+  for A :: "'a ty_absval_rel" and \<Lambda> :: var_context and  \<Gamma> :: "'a fun_context"
   where
-    RedAssertOk: "\<lbrakk> \<Gamma> \<turnstile> \<langle>e, n_s\<rangle> \<Down> (LBool True) \<rbrakk> \<Longrightarrow> 
-                 \<Lambda>,\<Gamma> \<turnstile> \<langle>Assert e, Normal n_s\<rangle> \<rightarrow> Normal n_s"
-  | RedAssertFail: "\<lbrakk> \<Gamma> \<turnstile> \<langle>e, n_s\<rangle> \<Down> (LBool False) \<rbrakk> \<Longrightarrow> 
-                  \<Lambda>,\<Gamma> \<turnstile> \<langle>Assert e, Normal n_s\<rangle> \<rightarrow> Failure"
-  | RedAssumeOk: "\<lbrakk> \<Gamma> \<turnstile> \<langle>e, n_s\<rangle> \<Down> (LBool True) \<rbrakk> \<Longrightarrow> 
-                \<Lambda>,\<Gamma> \<turnstile> \<langle>Assume e, Normal n_s\<rangle> \<rightarrow> Normal n_s"
-  | RedAssumeMagic: "\<lbrakk> \<Gamma> \<turnstile> \<langle>e, n_s\<rangle> \<Down> (LBool False) \<rbrakk> \<Longrightarrow> 
-                \<Lambda>,\<Gamma> \<turnstile> \<langle>Assume e, Normal n_s\<rangle> \<rightarrow> Magic"
-  | RedAssign: "\<lbrakk>\<Gamma> \<turnstile> \<langle>(map snd upds), n_s\<rangle> [\<Down>] vs \<rbrakk> \<Longrightarrow>
-               \<Lambda>,\<Gamma> \<turnstile> \<langle>Assign upds, Normal n_s\<rangle> \<rightarrow>  Normal (n_s((map fst upds) [\<mapsto>] vs))"  
+    RedAssertOk: "\<lbrakk> A,\<Gamma> \<turnstile> \<langle>e, n_s\<rangle> \<Down> LitV (LBool True) \<rbrakk> \<Longrightarrow> 
+                 A,\<Lambda>,\<Gamma> \<turnstile> \<langle>Assert e, Normal n_s\<rangle> \<rightarrow> Normal n_s"
+  | RedAssertFail: "\<lbrakk> A,\<Gamma> \<turnstile> \<langle>e, n_s\<rangle> \<Down> LitV (LBool False) \<rbrakk> \<Longrightarrow> 
+                  A,\<Lambda>,\<Gamma> \<turnstile> \<langle>Assert e, Normal n_s\<rangle> \<rightarrow> Failure"
+  | RedAssumeOk: "\<lbrakk> A,\<Gamma> \<turnstile> \<langle>e, n_s\<rangle> \<Down> LitV (LBool True) \<rbrakk> \<Longrightarrow> 
+                A,\<Lambda>,\<Gamma> \<turnstile> \<langle>Assume e, Normal n_s\<rangle> \<rightarrow> Normal n_s"
+  | RedAssumeMagic: "\<lbrakk> A,\<Gamma> \<turnstile> \<langle>e, n_s\<rangle> \<Down> LitV (LBool False) \<rbrakk> \<Longrightarrow> 
+                A,\<Lambda>,\<Gamma> \<turnstile> \<langle>Assume e, Normal n_s\<rangle> \<rightarrow> Magic"
+  | RedAssign: "\<lbrakk>A,\<Gamma> \<turnstile> \<langle>(map snd upds), n_s\<rangle> [\<Down>] vs \<rbrakk> \<Longrightarrow>
+               A,\<Lambda>,\<Gamma> \<turnstile> \<langle>Assign upds, Normal n_s\<rangle> \<rightarrow>  Normal (n_s((map fst upds) [\<mapsto>] vs))"  
   | RedHavoc: "\<lbrakk> map_of \<Lambda> x = Some ty; type_of_val v = ty \<rbrakk> \<Longrightarrow>
-               \<Lambda>,\<Gamma> \<turnstile> \<langle>Havoc x, Normal n_s\<rangle> \<rightarrow> Normal (n_s(x \<mapsto> v))"
-  | RedPropagateMagic: "\<Lambda>,\<Gamma> \<turnstile> \<langle>s, Magic\<rangle> \<rightarrow> Magic"
-  | RedPropagateFailure: "\<Lambda>,\<Gamma> \<turnstile> \<langle>s, Failure\<rangle> \<rightarrow> Failure"
+               A,\<Lambda>,\<Gamma> \<turnstile> \<langle>Havoc x, Normal n_s\<rangle> \<rightarrow> Normal (n_s(x \<mapsto> v))"
+  | RedPropagateMagic: "A,\<Lambda>,\<Gamma> \<turnstile> \<langle>s, Magic\<rangle> \<rightarrow> Magic"
+  | RedPropagateFailure: "A,\<Lambda>,\<Gamma> \<turnstile> \<langle>s, Failure\<rangle> \<rightarrow> Failure"
 
-inductive_cases RedAssertOk_case: "\<Lambda>,\<Gamma> \<turnstile> \<langle>Assert e, Normal n_s\<rangle> \<rightarrow> Normal n_s"
-inductive_cases RedAssumeOk_case: "\<Lambda>,\<Gamma> \<turnstile> \<langle>Assume e, Normal n_s\<rangle> \<rightarrow> Normal n_s"
+inductive_cases RedAssertOk_case: "A,\<Lambda>,\<Gamma> \<turnstile> \<langle>Assert e, Normal n_s\<rangle> \<rightarrow> Normal n_s"
+inductive_cases RedAssumeOk_case: "A,\<Lambda>,\<Gamma> \<turnstile> \<langle>Assume e, Normal n_s\<rangle> \<rightarrow> Normal n_s"
 
-inductive red_cmd_list :: "var_context \<Rightarrow> fun_context \<Rightarrow> cmd list \<Rightarrow> state \<Rightarrow> state \<Rightarrow> bool"
-  ("_,_ \<turnstile> ((\<langle>_,_\<rangle>) [\<rightarrow>]/ _)" [51,0,0,0] 81)
-  for \<Lambda> :: var_context and \<Gamma> :: fun_context
+inductive red_cmd_list :: "'a ty_absval_rel \<Rightarrow> var_context \<Rightarrow> 'a fun_context \<Rightarrow> cmd list \<Rightarrow> 'a state \<Rightarrow> 'a state \<Rightarrow> bool"
+  ("_,_,_ \<turnstile> ((\<langle>_,_\<rangle>) [\<rightarrow>]/ _)" [51,0,0,0] 81)
+  for A :: "'a ty_absval_rel" and \<Lambda> :: var_context and \<Gamma> :: "'a fun_context"
   where
-    RedCmdListNil: "\<Lambda>,\<Gamma> \<turnstile> \<langle>[],s\<rangle> [\<rightarrow>] s"
-  | RedCmdListCons: "\<lbrakk> \<Lambda>,\<Gamma> \<turnstile> \<langle>c,s\<rangle> \<rightarrow> s'; \<Lambda>,\<Gamma> \<turnstile> \<langle>cs,s'\<rangle> [\<rightarrow>] s'' \<rbrakk> \<Longrightarrow> 
-                   \<Lambda>,\<Gamma> \<turnstile> \<langle>(c # cs), s\<rangle> [\<rightarrow>] s''"
+    RedCmdListNil: "A,\<Lambda>,\<Gamma> \<turnstile> \<langle>[],s\<rangle> [\<rightarrow>] s"
+  | RedCmdListCons: "\<lbrakk> A,\<Lambda>,\<Gamma> \<turnstile> \<langle>c,s\<rangle> \<rightarrow> s'; A,\<Lambda>,\<Gamma> \<turnstile> \<langle>cs,s'\<rangle> [\<rightarrow>] s'' \<rbrakk> \<Longrightarrow> 
+                   A,\<Lambda>,\<Gamma> \<turnstile> \<langle>(c # cs), s\<rangle> [\<rightarrow>] s''"
 
-inductive_cases RedCmdListNil_case [elim]: "\<Lambda>,\<Gamma> \<turnstile> \<langle>[],s\<rangle> [\<rightarrow>] s"
-inductive_cases RedCmdListCons_case [elim]: "\<Lambda>,\<Gamma> \<turnstile> \<langle>(c # cs), s\<rangle> [\<rightarrow>] s''"
+thm red_cmd_list.induct
 
-type_synonym cfg_config = "(node+unit) \<times> state"
+inductive_cases RedCmdListNil_case [elim]: "A,\<Lambda>,\<Gamma> \<turnstile> \<langle>[],s\<rangle> [\<rightarrow>] s"
+inductive_cases RedCmdListCons_case [elim]: "A,\<Lambda>,\<Gamma> \<turnstile> \<langle>(c # cs), s\<rangle> [\<rightarrow>] s''"
 
-inductive red_cfg :: "var_context \<Rightarrow> fun_context \<Rightarrow> mbodyCFG \<Rightarrow> cfg_config \<Rightarrow> cfg_config \<Rightarrow> bool"
-  ("_,_,_ \<turnstile> (_ -n\<rightarrow>/ _)" [51,0,0,0] 81)
-  for \<Lambda> :: var_context and \<Gamma> :: fun_context and G :: mbodyCFG
+type_synonym 'a cfg_config = "(node+unit) \<times> 'a state"
+
+inductive red_cfg :: "'a ty_absval_rel \<Rightarrow> var_context \<Rightarrow> 'a fun_context \<Rightarrow> mbodyCFG \<Rightarrow> 'a cfg_config \<Rightarrow> 'a cfg_config \<Rightarrow> bool"
+  ("_,_,_,_ \<turnstile> (_ -n\<rightarrow>/ _)" [51,0,0,0] 81)
+  for A :: "'a ty_absval_rel" and \<Lambda> :: var_context and \<Gamma> :: "'a fun_context" and G :: mbodyCFG
   where
-    RedNode: "\<lbrakk>node_to_block(G) n = Some cs; \<Lambda>,\<Gamma> \<turnstile> \<langle>cs,s\<rangle> [\<rightarrow>] s'; n' \<in> out_edges(G) n  \<rbrakk> \<Longrightarrow> 
-              \<Lambda>, \<Gamma>, G  \<turnstile> (Inl n,s) -n\<rightarrow> (Inl n',s')"
-  | RedReturn: "\<lbrakk>node_to_block(G) n = Some cs; \<Lambda>, \<Gamma> \<turnstile> \<langle>cs,s\<rangle> [\<rightarrow>] s'; (out_edges(G) n) = {} \<rbrakk> \<Longrightarrow> 
-               \<Lambda>, \<Gamma>, G  \<turnstile> (Inl n,s) -n\<rightarrow> (Inr (),s')"
+    RedNode: "\<lbrakk>node_to_block(G) n = Some cs; A,\<Lambda>,\<Gamma> \<turnstile> \<langle>cs,s\<rangle> [\<rightarrow>] s'; n' \<in> out_edges(G) n  \<rbrakk> \<Longrightarrow> 
+              A,\<Lambda>,\<Gamma>,G  \<turnstile> (Inl n,s) -n\<rightarrow> (Inl n',s')"
+  | RedReturn: "\<lbrakk>node_to_block(G) n = Some cs; A,\<Lambda>,\<Gamma> \<turnstile> \<langle>cs,s\<rangle> [\<rightarrow>] s'; (out_edges(G) n) = {} \<rbrakk> \<Longrightarrow> 
+               A,\<Lambda>,\<Gamma>,G  \<turnstile> (Inl n,s) -n\<rightarrow> (Inr (),s')"
 
-inductive_cases RedNode_case: "\<Lambda>, \<Gamma>, G  \<turnstile> (Inl n,s) -n\<rightarrow> (Inl n',s')"
+inductive_cases RedNode_case: "A,\<Lambda>,\<Gamma>,G  \<turnstile> (Inl n,s) -n\<rightarrow> (Inl n',s')"
 
-abbreviation red_cfg_multi :: "var_context \<Rightarrow> fun_context \<Rightarrow> mbodyCFG \<Rightarrow> cfg_config \<Rightarrow> cfg_config \<Rightarrow> bool"
-  ("_,_,_ \<turnstile>_ -n\<rightarrow>*/ _" [51,0,0,0] 81)
-  where "red_cfg_multi \<Lambda> \<Gamma> G \<equiv> rtranclp (red_cfg \<Lambda> \<Gamma> G)"
+abbreviation red_cfg_multi :: "'a ty_absval_rel \<Rightarrow> var_context \<Rightarrow> 'a fun_context \<Rightarrow> mbodyCFG \<Rightarrow> 'a cfg_config \<Rightarrow> 'a cfg_config \<Rightarrow> bool"
+  ("_, _,_,_ \<turnstile>_ -n\<rightarrow>*/ _" [51,0,0,0] 81)
+  where "red_cfg_multi A \<Lambda> \<Gamma> G \<equiv> rtranclp (red_cfg A \<Lambda> \<Gamma> G)"
 
-abbreviation red_cfg_k_step :: "var_context \<Rightarrow> fun_context \<Rightarrow> mbodyCFG \<Rightarrow> cfg_config \<Rightarrow> nat \<Rightarrow> cfg_config \<Rightarrow> bool"
-  ("_,_,_ \<turnstile>_ -n\<rightarrow>^_/ _" [51,0,0,0,0] 81)
-where "red_cfg_k_step \<Lambda> \<Gamma> G c1 n c2 \<equiv> ((red_cfg \<Lambda> \<Gamma> G)^^n) c1 c2"
+abbreviation red_cfg_k_step :: "'a ty_absval_rel \<Rightarrow> var_context \<Rightarrow> 'a fun_context \<Rightarrow> mbodyCFG \<Rightarrow> 'a cfg_config \<Rightarrow> nat \<Rightarrow> 'a cfg_config \<Rightarrow> bool"
+  ("_,_,_,_ \<turnstile>_ -n\<rightarrow>^_/ _" [51,0,0,0,0] 81)
+where "red_cfg_k_step A \<Lambda> \<Gamma> G c1 n c2 \<equiv> ((red_cfg A \<Lambda> \<Gamma> G)^^n) c1 c2"
 
-fun fun_interp_single_wf :: "ty list \<times> ty \<Rightarrow> (val list \<rightharpoonup> val) \<Rightarrow> bool"
-  where "fun_interp_single_wf (args_ty, ret_ty) f =
-         (\<forall> vs. map type_of_val vs = args_ty \<longrightarrow> (\<exists>v. f vs = Some v \<and> type_of_val v = ret_ty)) "
+fun fun_interp_single_wf :: "'a ty_absval_rel \<Rightarrow> ty list \<times> ty \<Rightarrow> ('a val list \<rightharpoonup> 'a val) \<Rightarrow> bool"
+  where "fun_interp_single_wf A (args_ty, ret_ty) f =
+         (\<forall> vs. list_all (\<lambda> v_ty. ty_val_rel A (fst v_ty) (snd v_ty)) (zip vs args_ty) \<longrightarrow> 
+           (\<exists>v. f vs = Some v \<and> ty_val_rel A v ret_ty)) "
 
-definition fun_interp_wf :: "fdecls \<Rightarrow> fun_interp \<Rightarrow> bool"
-  where "fun_interp_wf fds \<gamma>_interp = 
+definition fun_interp_wf :: "'a ty_absval_rel \<Rightarrow> fdecls \<Rightarrow> 'a fun_interp \<Rightarrow> bool"
+  where "fun_interp_wf A fds \<gamma>_interp = 
             (\<forall>fn fd. map_of fds fn = Some fd \<longrightarrow> 
-                  (\<exists>f. \<gamma>_interp fn = Some f \<and> fun_interp_single_wf fd f ))"
+                  (\<exists>f. \<gamma>_interp fn = Some f \<and> fun_interp_single_wf A fd f ))"
 
-definition state_typ_wf :: "nstate \<Rightarrow> vdecls \<Rightarrow> bool"
-  where "state_typ_wf ns args = 
-           (\<forall> v v_ty. map_of args v = Some v_ty  \<longrightarrow> 
-                          Option.map_option type_of_val (ns(v)) = Some v_ty)"
+definition state_typ_wf :: "'a ty_absval_rel \<Rightarrow>'a nstate \<Rightarrow> vdecls \<Rightarrow> bool"
+  where "state_typ_wf A ns vs = 
+           (\<forall> v ty. map_of vs v = Some ty  \<longrightarrow> 
+                          Option.map_option (\<lambda>v. ty_val_rel A v ty)  (ns(v)) = Some True)"
 
-definition method_body_verifies :: "vdecls \<Rightarrow> fdecls \<Rightarrow> fun_interp \<Rightarrow> mbodyCFG \<Rightarrow> nstate \<Rightarrow> bool"
-  where "method_body_verifies vds fds \<gamma>_interp mbody ns = 
-      (\<forall> m' s'. (vds, (fds, \<gamma>_interp), mbody \<turnstile> (Inl (entry(mbody)), Normal ns) -n\<rightarrow>* (m',s')) \<longrightarrow> s' \<noteq> Failure)"
+definition method_body_verifies :: "'a ty_absval_rel \<Rightarrow> vdecls \<Rightarrow> fdecls \<Rightarrow> 'a fun_interp \<Rightarrow> mbodyCFG \<Rightarrow> 'a nstate \<Rightarrow> bool"
+  where "method_body_verifies A vds fds \<gamma>_interp mbody ns = 
+      (\<forall> m' s'. (A, vds, (fds, \<gamma>_interp), mbody \<turnstile> (Inl (entry(mbody)), Normal ns) -n\<rightarrow>* (m',s')) \<longrightarrow> s' \<noteq> Failure)"
 
-definition axiom_sat :: "fun_context \<Rightarrow> nstate \<Rightarrow> axiom \<Rightarrow> bool"
-  where "axiom_sat \<Gamma> n_s a = (\<Gamma> \<turnstile> \<langle>a, n_s\<rangle> \<Down> (LBool True))"
+definition axiom_sat :: "'a ty_absval_rel \<Rightarrow> 'a fun_context \<Rightarrow> 'a nstate \<Rightarrow> axiom \<Rightarrow> bool"
+  where "axiom_sat A \<Gamma> n_s a = (A,\<Gamma> \<turnstile> \<langle>a, n_s\<rangle> \<Down> LitV (LBool True))"
 
-definition axioms_sat :: "fun_context \<Rightarrow> nstate \<Rightarrow> axiom list \<Rightarrow> bool"
-  where "axioms_sat \<Gamma> n_s as = list_all (axiom_sat \<Gamma> n_s) as"
- 
+definition axioms_sat :: "'a ty_absval_rel \<Rightarrow> 'a fun_context \<Rightarrow> 'a nstate \<Rightarrow> axiom list \<Rightarrow> bool"
+  where "axioms_sat A \<Gamma> n_s as = list_all (axiom_sat A \<Gamma> n_s) as"
+
 (* not most compact representation (dom ns =... implied by ... state_typ wf ... ) *)
 (* disjointness condition does not reflect Boogie which allows shadowing of global variables *)
-fun method_verify :: "prog \<Rightarrow> mdecl \<Rightarrow> bool"
+fun method_verify :: "'a ty_absval_rel \<Rightarrow> prog \<Rightarrow> mdecl \<Rightarrow> bool"
   where 
-    "method_verify (Program fdecls consts gvars axioms mdecls) (mname, args, locals, mbody) =
-    (\<forall>\<gamma>_interp. fun_interp_wf fdecls \<gamma>_interp \<longrightarrow>
+    "method_verify A (Program fdecls consts gvars axioms mdecls) (mname, args, locals, mbody) =
+    (\<forall> \<gamma>_interp. fun_interp_wf A fdecls \<gamma>_interp \<longrightarrow>
      (\<forall>ns. 
-       (axioms_sat (fdecls, \<gamma>_interp) ns axioms) \<longrightarrow>
-       (state_typ_wf ns consts \<and> state_typ_wf ns gvars \<and> state_typ_wf ns args \<and> state_typ_wf ns locals) \<longrightarrow>
-        method_body_verifies (args@locals@gvars@consts) fdecls \<gamma>_interp mbody ns
+       (axioms_sat A (fdecls, \<gamma>_interp) ns axioms) \<longrightarrow>
+       (state_typ_wf A ns consts \<and> state_typ_wf A ns gvars \<and> state_typ_wf A ns args \<and> state_typ_wf A ns locals) \<longrightarrow>
+        method_body_verifies A (args@locals@gvars@consts) fdecls \<gamma>_interp mbody ns
       )
     )"
 
 lemma expr_eval_determ: 
-shows "((\<Gamma> \<turnstile> \<langle>e1, s\<rangle> \<Down> v) \<Longrightarrow> ((\<Gamma> \<turnstile> \<langle>e1, s\<rangle> \<Down> v') \<Longrightarrow> v = v'))"  
-    and "(\<Gamma> \<turnstile> \<langle>es, s\<rangle> [\<Down>] vs) \<Longrightarrow> (\<Gamma> \<turnstile> \<langle>es, s\<rangle> [\<Down>] vs') \<Longrightarrow> vs = vs' "
+shows "((A,\<Gamma> \<turnstile> \<langle>e1, s\<rangle> \<Down> v) \<Longrightarrow> ((A,\<Gamma> \<turnstile> \<langle>e1, s\<rangle> \<Down> v') \<Longrightarrow> v = v'))"  
+    and "(A,\<Gamma> \<turnstile> \<langle>es, s\<rangle> [\<Down>] vs) \<Longrightarrow> (A,\<Gamma> \<turnstile> \<langle>es, s\<rangle> [\<Down>] vs') \<Longrightarrow> vs = vs' "
 proof (induction arbitrary: v' and vs' rule: red_expr_red_exprs.inducts)
   case (RedVar n_s x v)
   assume "n_s x = Some v"
-  assume "\<Gamma> \<turnstile> \<langle>Var x,n_s\<rangle> \<Down> v'"
+  assume "A,\<Gamma> \<turnstile> \<langle>Var x,n_s\<rangle> \<Down> v'"
   then show ?case using \<open>n_s x = Some v\<close> by (cases; simp)
 next
-  case (RedVal v n_s)
-  assume "\<Gamma> \<turnstile> \<langle>Val v,n_s\<rangle> \<Down> v'"
+  case (RedLit l n_s)
+  assume "A,\<Gamma> \<turnstile> \<langle>Lit l,n_s\<rangle> \<Down> v'"
   then show ?case by (cases; simp)
 next
   case (RedBinOp e1 n_s v1 e2 v2 bop v)
   from RedBinOp.prems show ?case
   proof (cases)
     fix v1' v2'
-    assume "\<Gamma> \<turnstile> \<langle>e1,n_s\<rangle> \<Down> v1'" hence "v1 = v1'" using RedBinOp.IH by simp
-    assume "\<Gamma> \<turnstile> \<langle>e2,n_s\<rangle> \<Down> v2'" hence "v2 = v2'" using RedBinOp.IH by simp
-    assume "binop_eval bop v1' v2' = Some v'"
+    assume "A,\<Gamma> \<turnstile> \<langle>e1,n_s\<rangle> \<Down> v1'" hence "v1 = v1'" using RedBinOp.IH by simp
+    assume "A,\<Gamma> \<turnstile> \<langle>e2,n_s\<rangle> \<Down> v2'" hence "v2 = v2'" using RedBinOp.IH by simp
+    assume "binop_eval_val bop v1' v2' = Some v'"
     with \<open>v1 = v1'\<close> \<open>v2 = v2'\<close> show ?thesis using RedBinOp.hyps by simp
   qed
 next
@@ -283,8 +282,8 @@ next
   from RedUnOp.prems show ?case
   proof (cases)
     fix v2
-    assume "\<Gamma> \<turnstile> \<langle>e,n_s\<rangle> \<Down> v2" hence "v2 = v" using RedUnOp.IH by simp
-    assume "unop_eval uop v2 = Some veval"
+    assume "A,\<Gamma> \<turnstile> \<langle>e,n_s\<rangle> \<Down> v2" hence "v2 = v" using RedUnOp.IH by simp
+    assume "unop_eval_val uop v2 = Some veval"
     with \<open>v2 = v\<close> show ?thesis using RedUnOp.hyps by simp
   qed
 next
@@ -292,7 +291,7 @@ next
   from RedFunOp.prems show ?case
   proof (cases)
     fix v_args' f_interp'
-    assume "\<Gamma> \<turnstile> \<langle>args,n_s\<rangle> [\<Down>] v_args'" hence "v_args = v_args'" using RedFunOp.IH by simp
+    assume "A,\<Gamma> \<turnstile> \<langle>args,n_s\<rangle> [\<Down>] v_args'" hence "v_args = v_args'" using RedFunOp.IH by simp
     assume "snd \<Gamma> f = Some f_interp'" hence "f_interp = f_interp'" using RedFunOp.IH by simp
     assume "f_interp' v_args' = Some v'"
     thus ?case using \<open>v_args = v_args'\<close> \<open>f_interp = f_interp'\<close> using RedFunOp.hyps by simp
@@ -302,34 +301,34 @@ next
   thus ?case by (cases; simp)
 next
   case (RedExpListCons e n_s v es vs' vs'')
-  assume "\<Gamma> \<turnstile> \<langle>e # es,n_s\<rangle> [\<Down>] vs''"
+  assume "A,\<Gamma> \<turnstile> \<langle>e # es,n_s\<rangle> [\<Down>] vs''"
   thus ?case 
   proof cases
     fix w ws      
-    assume "\<Gamma> \<turnstile> \<langle>e,n_s\<rangle> \<Down> w" hence "v = w" using RedExpListCons.IH by simp
-    assume "\<Gamma> \<turnstile> \<langle>es,n_s\<rangle> [\<Down>] ws" hence "ws = vs'" using RedExpListCons.IH by simp  
+    assume "A,\<Gamma> \<turnstile> \<langle>e,n_s\<rangle> \<Down> w" hence "v = w" using RedExpListCons.IH by simp
+    assume "A,\<Gamma> \<turnstile> \<langle>es,n_s\<rangle> [\<Down>] ws" hence "ws = vs'" using RedExpListCons.IH by simp  
     moreover assume "vs'' = w # ws"
     ultimately show ?thesis using \<open>v = w\<close>  by simp
   qed
 next
   case (RedForAllTrue ty e n_s v')
-  from \<open>\<Gamma> \<turnstile> \<langle>Forall ty e,n_s\<rangle> \<Down> v'\<close>
+  from \<open>A,\<Gamma> \<turnstile> \<langle>Forall ty e,n_s\<rangle> \<Down> v'\<close>
   show ?case
   proof cases
     fix v''
-    assume "v' = LBool True"
+    assume "v' = LitV (LBool True)"
     thus ?thesis by simp
   next
     fix v''
-    assume "v' = LBool False"
-    assume "type_of_val v'' = ty"
-    moreover assume "\<Gamma> \<turnstile> \<langle>eopen 0 (Val v'') e,n_s\<rangle> \<Down> LBool False"
+    assume "v' = LitV (LBool False)"
+    assume "ty_val_rel A v'' ty"
+    moreover assume "A,\<Gamma> \<turnstile> \<langle>e, (shift n_s)(0 \<mapsto> v'')\<rangle> \<Down> LitV (LBool False)"
     ultimately show ?thesis using RedForAllTrue.IH(2)
-      by auto
+      by blast
   qed
 next
   case (RedForAllFalse v ty e n_s v')
-  from \<open>\<Gamma> \<turnstile> \<langle>Forall ty e,n_s\<rangle> \<Down> v'\<close>
+  from \<open>A,\<Gamma> \<turnstile> \<langle>Forall ty e,n_s\<rangle> \<Down> v'\<close>
   show ?case
   proof cases
     case RedForAllTrue
@@ -340,23 +339,23 @@ next
   qed
 next
   case (RedExistsTrue v ty e n_s v')
-  assume Hty:"type_of_val v = ty"
-  from \<open>\<Gamma> \<turnstile> \<langle>Exists ty e,n_s\<rangle> \<Down> v'\<close>
+  assume Hty:"ty_val_rel A v ty"
+  from \<open>A,\<Gamma> \<turnstile> \<langle>Exists ty e,n_s\<rangle> \<Down> v'\<close>
   show ?case
   proof cases
     case (RedExistsTrue v'')
     thus ?thesis by simp
   next
     case RedExistsFalse
-    with Hty have "\<Gamma> \<turnstile> \<langle>eopen 0 (Val v) e,n_s\<rangle> \<Down> LBool False" by simp
-    thus ?thesis using RedExistsTrue.IH by auto
+    with Hty have "A,\<Gamma> \<turnstile> \<langle>e, (shift n_s)(0 \<mapsto> v)\<rangle> \<Down> LitV (LBool False)" by simp
+    thus ?thesis using RedExistsTrue.IH by blast
   qed
 next
   case (RedExistsFalse ty e n_s v')
-  from \<open>\<Gamma> \<turnstile> \<langle>Exists ty e, n_s\<rangle> \<Down> v'\<close> show ?case
+  from \<open>A,\<Gamma> \<turnstile> \<langle>Exists ty e, n_s\<rangle> \<Down> v'\<close> show ?case
   proof cases
     case (RedExistsTrue v'')
-    thus ?thesis using RedExistsFalse.IH by auto
+    thus ?thesis using RedExistsFalse.IH by blast
   next
     case RedExistsFalse
     thus ?thesis by simp
@@ -364,7 +363,7 @@ next
 qed
 
 lemma step_nil_same:
-  assumes A1: "\<Lambda>,\<Gamma> \<turnstile> \<langle>[], s\<rangle> [\<rightarrow>] s''"
+  assumes A1: "A,\<Lambda>,\<Gamma> \<turnstile> \<langle>[], s\<rangle> [\<rightarrow>] s''"
   shows "s = s''"
 proof -
   from A1 show ?thesis by (cases; auto)
@@ -372,21 +371,21 @@ qed
 
 lemma no_out_edges_return:
   assumes 
-    A1: "\<Lambda>, \<Gamma>, G \<turnstile> (Inl n,s) -n\<rightarrow> (Inl n', s')" and 
+    A1: "A, \<Lambda>, \<Gamma>, G \<turnstile> (Inl n,s) -n\<rightarrow> (Inl n', s')" and 
     A2: "(out_edges(G) n) = {}"
   shows False
-  using A1 A2 red_cfg.simps by auto
+  using A1 A2 red_cfg.simps by blast
 
 lemma magic_stays_cmd:
-  assumes "\<Lambda>,\<Gamma> \<turnstile> \<langle>c, Magic\<rangle> \<rightarrow> s'"
+  assumes "A,\<Lambda>,\<Gamma> \<turnstile> \<langle>c, Magic\<rangle> \<rightarrow> s'"
   shows "s' = Magic"
   using assms
   by (cases rule: red_cmd.cases)
 
 lemma magic_stays_cmd_list:
-  assumes "\<Lambda>,\<Gamma> \<turnstile> \<langle>cs, Magic\<rangle> [\<rightarrow>] s'"
-  shows   " s' = Magic"
-  using assms 
+  assumes "A,\<Lambda>,\<Gamma> \<turnstile> \<langle>cs, Magic\<rangle> [\<rightarrow>] s'"
+  shows   "s' = Magic"
+  using assms
 proof (induction cs Magic s' rule: red_cmd_list.induct)
   case RedCmdListNil
   then show ?case by simp
@@ -396,20 +395,20 @@ next
 qed
 
 lemma magic_stays_cfg:
-  assumes "\<Lambda>, \<Gamma>, G \<turnstile> (m, Magic) -n\<rightarrow> (m', s')"
+  assumes "A, \<Lambda>, \<Gamma>, G \<turnstile> (m, Magic) -n\<rightarrow> (m', s')"
   shows " s' = Magic"
   using assms
 proof (cases rule: red_cfg.cases)
   case (RedNode n cs n')
-  then show ?thesis using magic_stays_cmd_list by simp
+  then show ?thesis using magic_stays_cmd_list by blast
 next
   case (RedReturn n cs)
-  then show ?thesis using magic_stays_cmd_list by simp
+  then show ?thesis using magic_stays_cmd_list by blast
 qed
 
 lemma magic_stays_cfg_multi:
   assumes
-    "\<Lambda>, \<Gamma>, G \<turnstile> (m, Magic) -n\<rightarrow>* (m', s')"
+    "A, \<Lambda>, \<Gamma>, G \<turnstile> (m, Magic) -n\<rightarrow>* (m', s')"
   shows "s' = Magic"
   using assms
 proof (induction rule: rtranclp_induct2)
@@ -422,13 +421,13 @@ qed
 
 lemma magic_stays_cfg_k_step:
   assumes
-    "\<Lambda>, \<Gamma>, G \<turnstile> (m, Magic) -n\<rightarrow>^k (m', s')"
+    "A, \<Lambda>, \<Gamma>, G \<turnstile> (m, Magic) -n\<rightarrow>^k (m', s')"
   shows "s' = Magic"
   using assms
   by (meson magic_stays_cfg_multi relpowp_imp_rtranclp)
 
 lemma finished_remains: 
-  assumes "\<Lambda>, \<Gamma>, G \<turnstile> (Inr (), n_s) -n\<rightarrow>* (m',n')"
+  assumes "A, \<Lambda>, \<Gamma>, G \<turnstile> (Inr (), n_s) -n\<rightarrow>* (m',n')"
   shows "(m',n') = (Inr(), n_s)"
   using assms
 proof (induction rule: rtranclp_induct2)
@@ -441,8 +440,8 @@ next
 qed
 
 lemma forall_red:
-  assumes "\<Gamma> \<turnstile> \<langle>Forall ty e, n_s\<rangle> \<Down> v"
-  shows "\<exists>b. (v = LBool b) \<and> (b = (\<forall>v'. type_of_val v' = ty \<longrightarrow> \<Gamma> \<turnstile> \<langle>eopen 0 (Val v') e, n_s\<rangle> \<Down> LBool True))"
+  assumes "A, \<Gamma> \<turnstile> \<langle>Forall ty e, n_s\<rangle> \<Down> v"
+  shows "\<exists>b. (v = LitV (LBool b)) \<and> (b = (\<forall>v'. ty_val_rel A v' ty \<longrightarrow> A, \<Gamma> \<turnstile> \<langle>e, (shift n_s)(0 \<mapsto> v')\<rangle> \<Down> LitV (LBool True)))"
   using assms
 proof (cases)
   case RedForAllTrue
@@ -454,8 +453,8 @@ next
 qed
 
 lemma exists_red:
-  assumes "\<Gamma> \<turnstile> \<langle>Forall ty e, n_s\<rangle> \<Down> v"
-  shows "\<exists>b. (v = LBool b) \<and> (b = (\<forall>v'. type_of_val v' = ty \<longrightarrow> \<Gamma> \<turnstile> \<langle>eopen 0 (Val v') e, n_s\<rangle> \<Down> LBool True))"
+  assumes "A, \<Gamma> \<turnstile> \<langle>Forall ty e, n_s\<rangle> \<Down> v"
+  shows "\<exists>b. (v = LitV (LBool b)) \<and> (b = (\<forall>v'. ty_val_rel A v' ty \<longrightarrow> A,\<Gamma> \<turnstile> \<langle>e, (shift n_s)(0 \<mapsto> v')\<rangle> \<Down> LitV (LBool True)))"
   using assms
 proof (cases)
   case RedForAllTrue
